

H.W

Q.1) Show that $(1+x)^x = 1 + x^2 - \frac{x^3}{2} + \frac{5x^4}{6} + \dots$

Ans \rightarrow let $y = (1+x)^n$
 $\therefore \log y = n \log(1+x)$

$\therefore e^{n \log(1+x)} = y$

$\therefore y = e^n \cdot e^{\log(1+x)}$

$\therefore y = e^n \cdot (1+x)$

$\therefore y = (1+x) \cdot \left[1 + \frac{x}{1!} + \frac{x^2}{2!} + \frac{x^3}{3!} + \dots \right]$

by using $(1+x)^m$

$= 1 + mn + \frac{m(m-1)}{2!}x^2 + \frac{m(m-1)(m-2)}{3!}x^3 + \dots$

$\therefore y = 1 + n \cdot x + \frac{n(n-1)}{2}x^2 + \dots$

$\therefore y = 1 + x^2 + \frac{(n-1)x^3}{2} + \dots$

$\therefore y = 1 + x^2 + \frac{x^4}{2} - \frac{x^5}{2} + \dots$

$\therefore y = 1 + x^2 - \frac{x^3}{2} + \dots$

$$\therefore y = \left(1 + x + \frac{x^2}{2!} + \frac{x^3}{3!} + \dots\right) + x \left(1 + x + \frac{x^2}{2!} + \frac{x^3}{3!} + \dots\right)$$

$$y = 1 + x + \frac{x^2}{2} + \frac{x^3}{6} + x + x^2 + \frac{x^3}{2} + \frac{x^4}{6} + \dots$$

$$y = 1 + 2x + \frac{3x^2}{2} + \frac{4x^3}{6} + \frac{x^4}{6} + \dots$$

$$y = 1 + 2x + \frac{3x^2}{2} + \frac{2x^3}{3} + \frac{x^4}{6} + \dots$$

Q.2) prove that $e^{e^x} = e \left[1 + x + \frac{x^2}{2} + \frac{5x^3}{6} + \dots \right]$

So let $y = e^{e^x}$

$$\therefore \log y = e^x \cdot \log_e e$$

$$\log y = e^x$$

$$\therefore \frac{1}{y} \times y' = e^x$$

$$y' = y \cdot e^x = e^{e^x} \cdot e^x = e^{(e^x + 1)}$$

let $f(x) = e^{e^x}$

$$\therefore f'(0) = e^{e^0} = e^1 = e$$

$$\therefore f'(0) = e^{e^0} \cdot e^0 = e^1 = e$$

$$\begin{aligned} \therefore f''(0) &= \frac{d}{dx} \left(e^{(e^x + x)} \right) = e^{(e^x + x)} (e^x + 1) \\ &= e^{(1+1)} (2) = 2e \end{aligned}$$

$$\begin{aligned}
 \therefore f'''(0) &= \frac{d}{dx} [e^{(e^x+x)} \cdot (e^x+1)] \\
 &= (e^x) \cdot e^{(e^x+x)} + (e^x+1) e^{(e^x+x)} (e^x+1) \\
 &= 1 \cdot e' + (2) e' (2) \\
 &= e + 4e \\
 &= 5e
 \end{aligned}$$

$$\begin{aligned}
 \therefore f(x) &= f(0) + x f'(0) + \frac{x^2}{2!} f''(0) + \frac{x^3}{3!} f'''(0) + \dots \\
 &= e + xe + \frac{x^2}{2} (2e) + \frac{x^3}{6} \times 5e + \dots \\
 &= e \left[1 + x + x^2 + \frac{5}{6} x^3 + \dots \right]
 \end{aligned}$$

Q.3 > prove that $x \cdot \operatorname{cosec} x = 1 + \frac{x^2}{6} + \frac{7}{360} x^4 + \dots$

Ans → here Instead of finding $x \cdot \operatorname{cosec} x$ will find only $\operatorname{cosec} x$

$$\therefore \text{let } f(x) = \operatorname{cosec} x$$

$$\therefore f(0) = \operatorname{cosec} 0 = \text{N.D}$$

$$\therefore f'(0) = -\cot(x) \cdot \operatorname{cosec}(x) = \text{N.D}$$

$$\therefore \text{let } x \cdot \operatorname{cosec} x = \frac{x}{\sin x}$$

$$\begin{aligned}
 \therefore \frac{x}{\sin x} &= \frac{x}{x - \frac{x^3}{3!} + \frac{x^5}{5!} - \frac{x^7}{7!} + \dots} = \frac{1}{1 - \frac{x^2}{3!} + \frac{x^4}{5!} - \frac{x^6}{7!} + \dots}
 \end{aligned}$$

$$e_0 = \frac{1}{1 - \left(\frac{x^2}{3!} - \frac{x^4}{5!} + \frac{x^6}{7!} - \frac{x^8}{9!} + \dots \right)}$$

by using $\left(\frac{1}{1-x} \right) = 1 + x + x^2 + x^3 + \dots$

$$e_0 = 1 + \left(\frac{x^2}{3!} - \frac{x^4}{5!} + \frac{x^6}{7!} - \dots \right) + \left(\frac{x^2}{3!} - \frac{x^4}{5!} + \frac{x^6}{7!} - \dots \right)^2 + \dots$$

$$= 1 + \frac{x^2}{3!} - \frac{x^4}{5!} + \dots + \frac{(84x)^2}{(5040)^2} x^4 + \dots$$

$$= 1 + \frac{x^2}{6} - \frac{x^4}{120} + \frac{7^2}{(42)^2} x^4 + \dots$$

$$= 1 + \frac{x^2}{6} - \frac{x^4}{120} + \frac{49}{1764} x^4 + \dots$$

$$= 1 + \frac{x^2}{6} - \frac{7}{360} x^4 + \dots$$

Q.4) prove that $\log \left(\frac{\sinh x}{x} \right) = \frac{x^2}{6} - \frac{x^4}{180} + \dots$

Ans →

let $y = \log \left(\frac{\sinh x}{x} \right)$

$$y = \log \left(\frac{x + \frac{x^3}{3!} + \frac{x^5}{5!} + \dots}{x} \right)$$

$$y = \log \left(1 + \frac{x^2}{3!} + \frac{x^4}{5!} + \dots \right)$$

∴ $y \neq \log(1/x) \neq 1$

by using $\log(1+x) = x - \frac{x^2}{2} + \frac{x^3}{3} - \frac{x^4}{4} \dots$

$$\therefore y = \left(\frac{x^2}{3!} + \frac{x^4}{5!} + \dots \right) - \frac{1}{2} \left(\frac{x^2}{3!} + \frac{x^4}{5!} + \dots \right)^2 \dots$$

$$\therefore y = \left(\frac{x^2}{3!} + \frac{x^4}{5!} + \dots \right) - \frac{1}{2} \left[\frac{x^4}{3! \times 3!} \dots \right]$$

$$y = \frac{x^2}{3!} + \frac{x^4}{5!} - \frac{x^4}{2 \times 3! \times 3!} \dots$$

$$y = \frac{x^2}{6} + \frac{x^4}{120} - \frac{x^4}{72} \dots$$

$$y = \frac{x^2}{6} - \frac{x^4}{180} \dots$$

Q.5) Prove that $\tan^{-1}x = x - \frac{x^3}{3} + \frac{x^5}{5} - \frac{x^7}{7} + \dots$

Ans → Let $f(x) = \tan^{-1}x$

$$\therefore f(0) = \tan^{-1}(0) = 0$$

$$\therefore f'(0) = \frac{1}{1+x^2} = 1$$

$$\therefore f''(0) = \frac{-1}{(1+x^2)^2} (2x) = 0$$

$$\therefore f'''(0) = \frac{-2(1+x^2)^2 + (2x)^2(1+x^2)(2x)}{(1+x^2)^2}$$

$$\therefore f'''(0) = \frac{-2 + 0}{1} = -2$$

$$\begin{aligned}\therefore f(x) &= f(0) + x f'(0) + \frac{x^2 f''(0)}{2} + \frac{x^3 f'''(0)}{6} - \dots \\ &= 0 + x(1) + 0 - \frac{x^3 \times (-2)}{6} - \dots \\ &= x - \frac{x^3}{3} + \dots\end{aligned}$$